Proof of the first texan triple!

theories/program_logic/itree_examples.v
@@ -1,5 +1,7 @@
 From stdpp Require Import base. 
-From shiris.program_logic Require Import itree evaluation itreewp.
+From iris.proofmode Require Import proofmode.
+From iris.base_logic.lib Require Import invariants.
+From shiris.program_logic Require Import evaluation heapmodel itree itreewp.
 
 Definition prog_swap  (l k: nat): expr nat unit := 
     x ← itree.get l ;
@@ -11,3 +13,64 @@ Definition loop_body {A}: unit -> expr nat A :=
 
 Definition loop_prog {A}: expr nat A :=
     loop_body ().
+
+Variant cell :=
+|Locked
+|UnLocked.
+
+Definition new_lock: expr cell loc :=
+  alloc UnLocked.
+
+Definition try_aquire (l: loc): expr cell bool :=
+  snd <$> cmpXchg l UnLocked Locked.
+
+Definition aqcuire_body (acq: bool): expr cell (() + ()) :=
+  if acq then mret $ inr $ () else mret $ inl $ ().
+
+Definition acquire (l: loc): expr cell () :=
+  itree.iter 
+    (λ _, try_aquire l ≫= aqcuire_body)  
+    tt.
+
+(* Definition acquire' (l: loc): expr cell () :=
+  itree.iter 
+    (λ _, try_aquire l ≫= (λ acq, if acq then mret $ inr $ () else mret $ inl $ ()))  
+    tt. *)
+
+Definition release (l: loc): expr cell () :=
+  put l UnLocked.
+
+Section lock_verification.
+  Context `{! inG Σ (heapR cell)}.
+  Context `{! invGS Σ}.
+  Context {γ: gname}.
+
+  Definition lock_inv (l: loc) (R: iProp Σ): iProp Σ :=
+    (∃ c: cell, 
+      points_to γ l c ∗
+      match c with
+      | Locked => True
+      | UnLocked => R
+      end
+    )%I.
+
+  Definition lockN: namespace := nroot .@ "lock".
+
+  Definition is_lock (l: loc) (R: iProp Σ): iProp Σ :=
+    inv lockN (lock_inv l R).
+    
+  (*
+    texan triple
+    ∀ Φ, P -∗ (Q -∗ Φ v) -∗ WP e {{ v, Φ v }}
+  *)
+  Lemma new_lock_spec (Φ: loc -> iProp Σ) (R: iProp Σ) (E: coPset):
+    R -∗ (∀l, is_lock l R -∗ Φ l) -∗ wp (state_interp γ) E new_lock (Φ).
+  Proof.
+    iIntros "R Hpost". iApply wp_fupd.
+    iApply wp_alloc. iIntros (l) "Hpt".
+    iMod (inv_alloc lockN _ (lock_inv l R) with "[R Hpt]") as "Hinv".
+    - iNext. iExists UnLocked. iFrame.
+    - iModIntro. iApply ("Hpost"). done.
+  Qed.
+
+End lock_verification.
